Lots of testing with tip-spec and fixed so that conjectures split over several lines gets parsed correctly when read back

Examples/SmallListDemo.thy
@@ -2,10 +2,6 @@ theory SmallListDemo
 imports "$HIPSTER_HOME/IsaHipster"
 begin
 
-(* Currently works poorly: Don't seem to get Sledgehammer to pick up theorems that's been 
-   discovered during the same theory exploration round.
- *) 
-
 datatype 'a Lst = 
   Emp
   | Cons "'a" "'a Lst"
@@ -15,35 +11,78 @@ where
   "app Emp xs = xs"
 | "app (Cons x xs) ys = Cons x (app xs ys)"
 
+hipster app
+lemma lemma_a [thy_expl]: "app y Emp = y"
+apply (induction y)
+apply simp
+by simp
+
+lemma lemma_aa [thy_expl]: "app (app y z) x2 = app y (app z x2)"
+apply (induction y)
+apply simp
+by simp
+
 fun rev :: "'a Lst \<Rightarrow> 'a Lst"
 where 
   "rev Emp = Emp"
 | "rev (Cons x xs) = app (rev xs) (Cons x Emp)"
 
-hipster app
-
-lemma lemma_a [thy_expl]: "app x Emp = x"
-apply (induction x)
+fun len ::  "'a Lst \<Rightarrow> nat"
+where
+  "len Emp = 0"
+| "len (Cons x xs) = 1 + (len xs)"  
+hipster app len
+lemma lemma_ab [thy_expl]: "len y + len z = len (app y z)"
+apply (induction y)
 apply simp
 by simp
 
-lemma lemma_aa [thy_expl]: "app (app x y) z = app x (app y z)"
-apply (induction x)
+lemma lemma_ac [thy_expl]: "len (app z y) = len (app y z)"
+apply (induction y)
+apply simp
+apply (metis lemma_a)
+apply simp
+by (metis SmallListDemo.lemma_ab Suc_eq_plus1_left add.left_commute len.simps(2))
+
+fun filt :: "('a \<Rightarrow> bool) \<Rightarrow> 'a Lst \<Rightarrow> 'a Lst" 
+where 
+  "filt p Emp = Emp"
+| "filt p (Cons x xs) = (if (p x) then (Cons x (filt p xs)) else (filt p xs))"
+
+fun mem :: "'a \<Rightarrow> 'a Lst \<Rightarrow> bool"
+where
+  "mem x Emp = False"
+| "mem x (Cons y ys) = ((x=y) \<or> (mem x ys))"
+
+hipster app filt
+lemma lemma_ad [thy_expl]: "filt y (filt y z) = filt y z"
+apply (induction z)
 apply simp
 by simp
+
+lemma lemma_ae [thy_expl]: "filt z (filt y x2) = filt y (filt z x2)"
+apply (induction x2)
+apply simp
+by simp
+
+lemma lemma_af [thy_expl]: "app (filt y z) (filt y x2) = filt y (app z x2)"
+apply (induction z)
+apply simp
+by simp
+
 hipster rev
-lemma lemma_ab [thy_expl]: "app (SmallListDemo.rev x) (SmallListDemo.rev y) =
-SmallListDemo.rev (app y x)"
+lemma lemma_ag [thy_expl]: "app (SmallListDemo.rev z) (SmallListDemo.rev y) =
+SmallListDemo.rev (app y z)"
 apply (induction y)
 apply simp
 apply (metis lemma_a)
 apply simp
 by (metis lemma_aa)
 
-lemma lemma_ac [thy_expl]: "SmallListDemo.rev (SmallListDemo.rev x) = x"
-apply (induction x)
+lemma lemma_ah [thy_expl]: "SmallListDemo.rev (SmallListDemo.rev y) = y"
+apply (induction y)
 apply simp
 apply simp
-by (metis Lst.distinct(1) SmallListDemo.rev.simps(1) SmallListDemo.rev.simps(2) app.elims app.simps(2) lemma_a lemma_ab)
+by (metis Lst.distinct(1) SmallListDemo.rev.simps(1) SmallListDemo.rev.simps(2) app.elims app.simps(2) lemma_a lemma_ag)
 
 end
