IsaHipster.thy
@@ -31,7 +31,7 @@ val haskell_path =
 val hipspecifyer_cmd = haskell_path ^ "HipSpecifyer "; 
 *)
 val tipSpec_cmd = haskell_path ^ "tip-spec ";
-val tip_cmd = haskell_path ^ "tip --hipster ";
+val tipTransl_cmd = haskell_path ^ "tip --hipster ";
 val tipGHC_cmd = haskell_path ^ "tip-ghc ";
 end
 
@@ -93,7 +93,8 @@ method_setup hipster_induct = {*
   Scan.lift (Scan.succeed 
     (fn ctxt => SIMPLE_METHOD 
       (Induct_CTac.hipster_induct ctxt)))
-   *}
+   *}  
+
 (*
 ML{*
 Method.setup;
